Arithmetization/ISigmaOne/Ind.lean
@@ -12,12 +12,11 @@ namespace LO.Arith
 
 open FirstOrder FirstOrder.Arith
 
-variable {V : Type*} [Zero V] [One V] [Add V] [Mul V] [LT V]
-
+variable {V : Type*} [ORingStruc V]
 
 variable (m : ℕ) [Fact (1 ≤ m)] [V ⊧ₘ* 𝐈𝐍𝐃𝚺 m]
 
-lemma induction_sigma_or_pi {P Q : V → Prop} (hP : (𝚺, m)-Predicate P) (hQ : (𝚷, m)-Predicate Q)
+lemma induction_sigma_or_pi {P Q : V → Prop} (hP : 𝚺-[m]-Predicate P) (hQ : 𝚷-[m]-Predicate Q)
     (zero : P 0 ∨ Q 0) (succ : ∀ x, P x ∨ Q x → P (x + 1) ∨ Q (x + 1)) : ∀ x, P x ∨ Q x := by
   haveI : V ⊧ₘ* 𝐈𝚺₁ := mod_ISigma_of_le (show 1 ≤ m from Fact.out)
   intro a
@@ -40,7 +39,7 @@ lemma induction_sigma_or_pi {P Q : V → Prop} (hP : (𝚺, m)-Predicate P) (hQ 
   have := this a (by rfl)
   simpa [hp, hq] using this
 
-lemma order_induction_sigma_or_pi {P Q : V → Prop} (hP : (𝚺, m)-Predicate P) (hQ : (𝚷, m)-Predicate Q)
+lemma order_induction_sigma_or_pi {P Q : V → Prop} (hP : 𝚺-[m]-Predicate P) (hQ : 𝚷-[m]-Predicate Q)
     (ind : ∀ x, (∀ y < x, P y ∨ Q y) → P x ∨ Q x) : ∀ x, P x ∨ Q x := by
   haveI : V ⊧ₘ* 𝐈𝚺₁ := mod_ISigma_of_le (show 1 ≤ m from Fact.out)
   intro a
@@ -56,17 +55,17 @@ lemma order_induction_sigma_or_pi {P Q : V → Prop} (hP : (𝚺, m)-Predicate P
     · clear hp hq ind
       apply LO.FirstOrder.Arith.HierarchySymbol.Boldface.imp
       · simp_all only [SigmaPiDelta.alt_sigma, Fin.isValue]
-        apply LO.FirstOrder.Arith.HierarchySymbol.Boldface.comp₂_infer
-        · simp_all only [zero_add, Fin.isValue, DefinableFunction.var]
-        · simp_all only [zero_add, DefinableFunction.const]
+        apply LO.FirstOrder.Arith.HierarchySymbol.Boldface.comp₂
+        · simp_all only [zero_add, Fin.isValue, HierarchySymbol.BoldfaceFunction.var]
+        · simp_all only [zero_add, HierarchySymbol.BoldfaceFunction.const]
       · simp_all only [Fin.isValue]
         apply LO.FirstOrder.Arith.HierarchySymbol.Boldface.or
-        · apply LO.FirstOrder.Arith.HierarchySymbol.Boldface.comp₂_infer
-          · simp_all only [zero_add, Fin.isValue, DefinableFunction.var]
-          · simp_all only [zero_add, DefinableFunction.const]
-        · apply LO.FirstOrder.Arith.HierarchySymbol.Boldface.comp₂_infer
-          · simp_all only [zero_add, Fin.isValue, DefinableFunction.var]
-          · simp_all only [zero_add, DefinableFunction.const]
+        · apply LO.FirstOrder.Arith.HierarchySymbol.Boldface.comp₂
+          · simp_all only [zero_add, Fin.isValue, HierarchySymbol.BoldfaceFunction.var]
+          · simp_all only [zero_add, HierarchySymbol.BoldfaceFunction.const]
+        · apply LO.FirstOrder.Arith.HierarchySymbol.Boldface.comp₂
+          · simp_all only [zero_add, Fin.isValue, HierarchySymbol.BoldfaceFunction.var]
+          · simp_all only [zero_add, HierarchySymbol.BoldfaceFunction.const]
     case ind z ih =>
       have : P z ∨ Q z :=
         ind z (fun y hy ↦ by
