Arithmetization/ISigmaOne/Metamath/Formula/Typed.lean
@@ -13,7 +13,7 @@ namespace LO.Arith
 
 open FirstOrder FirstOrder.Arith
 
-variable {V : Type*} [Zero V] [One V] [Add V] [Mul V] [LT V] [V ⊧ₘ* 𝐈𝚺₁]
+variable {V : Type*} [ORingStruc V] [V ⊧ₘ* 𝐈𝚺₁]
 
 variable {L : Arith.Language V} {pL : LDef} [Arith.Language.Defined L pL]
 
