Arithmetization/ISigmaOne/Metamath/Term/Typed.lean
@@ -12,7 +12,7 @@ namespace LO.Arith
 
 open FirstOrder FirstOrder.Arith
 
-variable {V : Type*} [Zero V] [One V] [Add V] [Mul V] [LT V] [V ⊧ₘ* 𝐈𝚺₁]
+variable {V : Type*} [ORingStruc V] [V ⊧ₘ* 𝐈𝚺₁]
 
 variable {L : Arith.Language V} {pL : LDef} [Arith.Language.Defined L pL]
 
@@ -278,7 +278,7 @@ instance (n : V) : Add (⌜ℒₒᵣ⌝.TSemiterm n) := ⟨add⟩
 
 instance (n : V) : Mul (⌜ℒₒᵣ⌝.TSemiterm n) := ⟨mul⟩
 
-instance (n : V) : Coe V (⌜ℒₒᵣ⌝.TSemiterm n) := ⟨typedNumeral n⟩
+instance coeNumeral (n : V) : Coe V (⌜ℒₒᵣ⌝.TSemiterm n) := ⟨typedNumeral n⟩
 
 variable {n : V}
 
